language_formalisation/syntax/syntax.v
@@ -146,46 +146,57 @@ match h with
 | CasesU h op x k c => (h_no_var_j h j) /\ (c_no_var_j c (2+j))
 end.
 
-Fixpoint v_under_var_j (v:val) (j:nat) :=
+Fixpoint v_under_var (v:val) (j:nat) :=
 match v with
 | Var (name, num) => num < j
 | Unit => True
 | Int j => True
-| Inl v' => v_under_var_j v' j
-| Inr v' => v_under_var_j v' j
-| Pair v1 v2 => (v_under_var_j v1 j) /\ (v_under_var_j v2 j)
-| Fun x c => c_under_var_j c (1+j)
-| Handler x c_ret h => (c_under_var_j c_ret (1+j)) /\ (h_under_var_j h j)
+| Inl v' => v_under_var v' j
+| Inr v' => v_under_var v' j
+| Pair v1 v2 => (v_under_var v1 j) /\ (v_under_var v2 j)
+| Fun x c => c_under_var c (1+j)
+| Handler x c_ret h => (c_under_var c_ret (1+j)) /\ (h_under_var h j)
 end
-with c_under_var_j (c:comp) (j:nat) :=
+with c_under_var (c:comp) (j:nat) :=
 match c with
-| Ret v => v_under_var_j v j
-| Absurd v => v_under_var_j v j 
-| ΠMatch v x y c => (v_under_var_j v j) /\ c_under_var_j c (2+j)
+| Ret v => v_under_var v j
+| Absurd v => v_under_var v j 
+| ΠMatch v x y c => (v_under_var v j) /\ c_under_var c (2+j)
 | ΣMatch v xl cl xr cr =>
-    (v_under_var_j v j) /\ (c_under_var_j cl (1+j)) /\ (c_under_var_j cr (1+j))
-| App v1 v2 => (v_under_var_j v1 j) /\ (v_under_var_j v2 j)
-| Op op v_arg y c => (v_under_var_j v_arg j) /\ (c_under_var_j c (1+j))
-| LetRec f x c1 c2 => (c_under_var_j c1 (2+j)) /\ (c_under_var_j c2 (1+j))
-| DoBind x c1 c2 => (c_under_var_j c1 j) /\ (c_under_var_j c2 (1+j))
-| Handle v c' => (v_under_var_j v j) /\ (c_under_var_j c' j)
+    (v_under_var v j) /\ (c_under_var cl (1+j)) /\ (c_under_var cr (1+j))
+| App v1 v2 => (v_under_var v1 j) /\ (v_under_var v2 j)
+| Op op v_arg y c => (v_under_var v_arg j) /\ (c_under_var c (1+j))
+| LetRec f x c1 c2 => (c_under_var c1 (2+j)) /\ (c_under_var c2 (1+j))
+| DoBind x c1 c2 => (c_under_var c1 j) /\ (c_under_var c2 (1+j))
+| Handle v c' => (v_under_var v j) /\ (c_under_var c' j)
 end
-with h_under_var_j (h:hcases) (j:nat) :=
+with h_under_var (h:hcases) (j:nat) :=
 match h with
 | CasesØ => True
-| CasesU h op x k c => (h_under_var_j h j) /\ (c_under_var_j c (2+j))
+| CasesU h op x k c => (h_under_var h j) /\ (c_under_var c (2+j))
 end.
 
-Fixpoint tmpl_under_var_j (T:tmpl) (j:nat) :=
+Fixpoint tmpl_under_var (T:tmpl) (j:nat) :=
 match T with
-| TApp (name, num) v => num < j /\ v_under_var_j v j
-| TAbsurd v => v_under_var_j v j
-| TΠMatch v x y T => v_under_var_j v j /\ tmpl_under_var_j T (2+j)
+| TApp (name, num) v => v_under_var v j
+| TAbsurd v => v_under_var v j
+| TΠMatch v x y T => v_under_var v j /\ tmpl_under_var T (2+j)
 | TΣMatch v xl Tl xr Tr =>
-    (v_under_var_j v j) /\ (tmpl_under_var_j Tl (1+j)) 
-    /\ (tmpl_under_var_j Tr (1+j))
-| TOp op v_arg y T => (v_under_var_j v_arg j) /\ (tmpl_under_var_j T (1+j))
+    (v_under_var v j) /\ (tmpl_under_var Tl (1+j)) 
+    /\ (tmpl_under_var Tr (1+j))
+| TOp op v_arg y T => (v_under_var v_arg j) /\ (tmpl_under_var T (1+j))
 end.
+
+Fixpoint tmpl_under_tvar_j (T:tmpl) (j:nat) :=
+match T with
+| TApp (name, num) v => num < j
+| TAbsurd v => True
+| TΠMatch v x y T => tmpl_under_tvar_j T j
+| TΣMatch v xl Tl xr Tr => 
+    (tmpl_under_tvar_j Tl j) /\ (tmpl_under_tvar_j Tr j)
+| TOp op v_arg y T => (tmpl_under_tvar_j T j)
+end.
+
 
 Fixpoint ctx_remove_var (Γ:ctx) (i:nat) :=
   match Γ, i with
